LabelPost fold

relabel/relabel.v
@@ -1,6 +1,6 @@
 Require Import MoSel.
 
-Import adequacy_gensym_SLMin.
+Import adequacy_gensym_SLList.
 
 Inductive Tree (X : Type) :=
 | Leaf : X -> Tree X
@@ -8,7 +8,6 @@ Inductive Tree (X : Type) :=
 
 Arguments Leaf {_}.
 Arguments Node {X}.
-
 
 Fixpoint label {X} (t : Tree X) : mon Fresh (Tree ident) :=
   match t with
@@ -23,40 +22,30 @@ Fixpoint label {X} (t : Tree X) : mon Fresh (Tree ident) :=
 
 Definition relabel {X} (t : Tree X): Tree ident := snd (run (label t) initial_state).
 
-Fixpoint labelPost {X} (t: Tree X) (t_res : Tree ident) : iProp :=
-  match t,t_res with
-  | Leaf _, Leaf v => IsFresh v
-  | Node l r, Node l_res r_res => labelPost l l_res ∗ labelPost r r_res
-  | _, _ => False
-  end.
-
-Lemma label_spec : forall X (t : Tree X),
-    ⊢ {{ emp }} label t {{ t'; labelPost t t' }}.
-Proof.
-  induction t.
-  - iBind. eapply gensym_spec. iRet.
-  - iBind. eapply IHt1. iBind. Frame. eapply IHt2. iRet. iIntros "[$ $]".
-Qed.
-
 Fixpoint flatten {X} (t: Tree X) : list X :=
   match t with
   | Leaf v => cons v nil
   | Node l r => flatten l ++ flatten r
   end.
 
-Definition sameShape {X Y} (t1 : Tree X) (t2 : Tree Y) : Prop :=
+Fixpoint sameShape {X Y} (t1 : Tree X) (t2 : Tree Y) : Prop :=
   match t1,t2 with
   | Leaf _, Leaf _ => True
-  | Node _ _, Node _ _  => True
+  | Node l r, Node l_res r_res  => sameShape l l_res /\ sameShape r r_res
   | _, _ => False
   end.
 
-Lemma labelpost_fold : forall X (t : Tree X) t',
-    ⊢ labelPost t t' -∗ [∗ list] x ∈ (flatten t'), IsFresh x.
+Definition labelPost {X} (t: Tree X) (t_res : Tree ident) : iProp :=
+  ([∗ list] x ∈ (flatten t_res), IsFresh x) ∗ ⌜sameShape t t_res⌝.
+
+Lemma label_spec : forall X (t : Tree X),
+    ⊢ {{ emp }} label t {{ t'; labelPost t t' }}.
 Proof.
-  induction t, t'; simpl; iIntros; norm_all; auto; try contradiction.
-  iDestruct (IHt1 with "HB") as "Ht1". iDestruct (IHt2 with "HC") as "Ht2".
-  iApply big_sepL_app. iFrame.
+  induction t.
+  - iBind. eapply gensym_spec. iRet. rewrite /labelPost. simpl; auto.
+  - simpl label. iBind. eapply IHt1. iBind. Frame. eapply IHt2. iRet.
+    rewrite /labelPost. iIntros "[[HA %] [HB %]]". iSplitL; auto.
+    simpl. iApply big_sepL_app. iFrame.
 Qed.
 
 Lemma sep_list_fold : forall a l, ⊢ (IsFresh a -∗ ([∗ list] x ∈ l, IsFresh x) -∗ ⌜a ∉ l⌝ : iProp).
@@ -78,24 +67,18 @@ Proof.
     iPureIntro. constructor; auto.
 Qed.
 
-Lemma labelpost_nodup : forall X (t : Tree X) t0,
-    ⊢ labelPost t t0 -∗ ⌜NoDup (flatten t0)⌝.
-Proof.
-  iIntros; norm_all. iDestruct (labelpost_fold with "HB") as "HB".
-  iDestruct (fold_nodup with "HB") as "$".
-Qed.
-
 Lemma finish_him : forall X (t : Tree X) t' h,
     labelPost t t' () h -> NoDup (flatten t') /\ sameShape t t'.
 Proof.
   intros. apply soundness3 in H. apply (soundness1 h).
-  iIntros "HA". iDestruct (H with "HA") as "HA". iDestruct (labelpost_nodup with "HA") as "%".
-  iSplit; auto. destruct t,t'; auto.
+  iIntros "HA". iDestruct (H with "HA") as "[HA HB]".
+  iDestruct (fold_nodup with "HA") as "HA". iSplit; auto.
 Qed.
 
 Lemma relabel_spec : forall X (t : Tree X) t',
     relabel t = t' -> NoDup (flatten t') /\ sameShape t t'.
 Proof.
   intros. unfold relabel in H. destruct (run (label t) initial_state) eqn:?. destruct H. simpl.
-  eapply (finish_him _ _ _ _ (adequacy_triple_init _ _ _ _ _ emp_trivial (label_spec _ t) Heqp)).
+  eapply finish_him. eapply adequacy_triple_init; eauto.
+  apply emp_trivial. apply label_spec.
 Qed.
